added ActionModel, working on single AM counterpart of EM

fairness/utils.v
@@ -700,3 +700,177 @@ Section ExtractSomes.
   Qed. 
 
 End ExtractSomes.
+
+
+Require Import ClassicalFacts.
+
+Lemma min_prop_dec_impl (P: nat -> Prop) (DEC: forall n, Decision (P n)):
+  ∀ n, P n → {m | Minimal P m}.
+Proof.
+  intros n Pn.
+
+  assert (forall p, p <= n + 1 -> ({m | Minimal P m} + {forall k, k < p -> ¬ P k})) as MIN'.
+  2: { destruct (MIN' (n + 1)); eauto. edestruct n0; eauto. lia. }
+
+  induction p.
+  { intros. right. lia. }
+  intros. destruct IHp; [lia| auto| ].
+  rewrite Nat.add_1_r in H. apply le_S_n in H. 
+  destruct (DEC p).
+  - left. exists p. split; auto. intros.
+    destruct (decide (p <= k)); auto.
+    destruct (n0 k); auto. lia.
+  - right. intros. destruct (decide (k = p)); [congruence| ].
+    apply n0. lia.
+Qed. 
+
+Definition Minimal_pos (P: positive → Prop) (n : positive) :=
+  P n ∧ (∀ k, P k → Pos.le n k). 
+
+Lemma min_prop_dec_impl_pos (P: positive -> Prop) (DEC: forall n, Decision (P n)):
+  ∀ n, P n → {m: positive | Minimal_pos P m }.
+Proof.
+  intros n Pn.
+  epose proof (min_prop_dec_impl (P ∘ Pos.of_nat) _ (Pos.to_nat n)) as [m [Pm MINm]].
+  { red. by rewrite Pos2Nat.id. }
+  exists (Pos.of_nat m). split; auto.
+  intros.
+  specialize (MINm (Pos.to_nat k) ltac:(red; by rewrite Pos2Nat.id)). 
+  lia. 
+Qed.
+
+From stdpp Require Import namespaces coPset. 
+Section CoPsetOrdering.
+  
+  Definition coPset_least (C: coPset) (INF: ¬ set_finite C) : positive :=
+    let c := coPpick C in
+    let m := min_prop_dec_impl_pos (fun p => p ∈ C) _ c (coPpick_elem_of _ INF) in
+    proj1_sig m.
+
+  Lemma coPset_least_spec (C: coPset) (INF: ¬ set_finite C):
+    Minimal_pos (fun p => p ∈ C) (coPset_least C INF).
+  Proof.
+    rewrite /coPset_least.
+    by destruct min_prop_dec_impl_pos.
+  Qed.
+
+  Lemma coPset_least_in (C: coPset) (INF: ¬ set_finite C):
+    coPset_least C INF ∈ C. 
+  Proof.
+    apply coPset_least_spec. 
+  Qed.
+
+  Local Lemma coPset_sub1_helper (C: coPset) (INF: ¬ set_finite C) (m: positive):
+    ¬ set_finite (C ∖ {[ m ]}).
+  Proof.
+    apply coPset_infinite_finite. apply difference_infinite.
+    - by apply coPset_infinite_finite.
+    - apply singleton_finite.
+  Qed. 
+
+  Fixpoint coPset_nth (C: coPset) (INF: ¬ set_finite C) (n: nat): positive :=
+    let m := coPset_least C INF in
+    match n with
+    | 0 => m
+    | S n => coPset_nth (C ∖ {[ m ]}) (coPset_sub1_helper C INF m) n
+    end.
+
+  Definition ns_nth (ns: namespace) :=
+    coPset_nth (↑ns) (nclose_infinite ns). 
+
+  Lemma coPset_nth_in C INF i:
+    coPset_nth C INF i ∈ C. 
+  Proof.
+    remember (coPset_nth C INF i) as c. generalize dependent c. 
+    generalize dependent C. induction i.
+    { simpl. intros. subst. apply coPset_least_in. }
+    simpl. intros.
+  (*   ospecialize * (IHi _ _). *)
+  (*   { apply Heqc. } *)
+  (*   set_solver. *)
+  (* Qed.  *)
+  Admitted. 
+
+  Lemma coPset_nth_disj_neq C1 C2 INF1 INF2 n1 n2
+    (DISJ: C1 ## C2):
+    coPset_nth C1 INF1 n1 ≠ coPset_nth C2 INF2 n2.
+  Proof. 
+    pose proof (coPset_nth_in _ INF1 n1).
+    pose proof (coPset_nth_in _ INF2 n2) as IN2. 
+    intros EQ. rewrite -EQ in IN2. set_solver.
+  Qed. 
+
+  Lemma coPset_nth_next_lt C INF i:
+    (coPset_nth C INF i < coPset_nth C INF (S i))%positive.
+  Proof.
+  (*   remember (coPset_nth C INF i) as m. remember (coPset_nth C INF (S i)) as m'. *)
+  (*   generalize dependent C. generalize dependent m. generalize dependent m'.  *)
+  (*   induction i. *)
+  (*   { simpl. intros. *)
+  (*     pose proof (coPset_least_spec C INF). *)
+  (*     assert (m' ∈ C) as IN'. *)
+  (*     { subst m'. eapply elem_of_weaken; [apply coPset_least_in| ]. set_solver. } *)
+  (*     red in H. apply proj2 in H. ospecialize (H m' IN'). *)
+  (*     rewrite -Heqm in H. apply Positive_as_OT.le_lteq in H as [? | ?]; [lia| ]. *)
+  (*     rewrite -Heqm in Heqm'. *)
+  (*     pose proof (coPset_least_in _ (coPset_sub1_helper C INF m)). *)
+  (*     set_solver. } *)
+  (*   intros. *)
+  (*   pose proof (coPset_sub1_helper C INF (coPset_least C INF)) as INF'. *)
+  (*   eapply IHi; eauto.  *)
+  (* Qed.  *)
+  Admitted. 
+
+  Lemma coPset_nth_lt C INF i j (LT: i < j):
+    (coPset_nth C INF i < coPset_nth C INF j)%positive.
+  Proof.
+    apply Nat.lt_exists_pred in LT as (? & -> & LE).
+    apply Nat.le_sum in LE as [d ->]. 
+    induction d.
+    { rewrite Nat.add_0_r. apply coPset_nth_next_lt. }
+    etrans; eauto.
+    eapply Positive_as_OT.lt_le_trans; [apply coPset_nth_next_lt| ].
+    apply Positive_as_OT.le_lteq. right. f_equal. lia.
+  Qed.     
+
+  Lemma coPset_nth_inj (C: coPset) (INF: ¬ set_finite C):
+    Inj eq eq (coPset_nth C INF).
+  Proof.
+    red. intros i j EQ.
+    destruct (Nat.lt_trichotomy i j) as [LT|[?|LT]]; auto.
+    all: apply (coPset_nth_lt C INF) in LT; lia.
+  Qed.
+
+  Lemma coPset_nth_surj (C: coPset) (INF: ¬ set_finite C):
+    forall p, p ∈ C -> exists n, p = coPset_nth C INF n. 
+  Proof.
+    intros p INp. 
+    remember (coPset_least C INF) as m.
+    remember (Pos.to_nat p - Pos.to_nat m) as d.
+    generalize dependent m. generalize dependent C.
+    pattern d. apply lt_wf_ind. clear d. intros d IH.     
+    destruct (decide (d = 0)) as [-> | NZ]. 
+    { simpl. intros. symmetry in Heqd. apply Nat.sub_0_le in Heqd.
+      apply Pos2Nat.inj_le in Heqd.
+      apply Positive_as_OT.le_lteq in Heqd as [LT | ->].
+      2: { by exists 0. }
+      pose proof (coPset_least_spec C INF). rewrite -Heqm in H.
+      red in H. apply proj2 in H. specialize (H _ INp). 
+      lia. }
+    intros.
+    set (m' := coPset_least (C ∖ {[ m ]}) (coPset_sub1_helper C INF m)).
+    assert (m' ∈ C ∖ {[ m ]}) as IN'.
+    { subst m'. apply coPset_least_in. }
+  (*   ospecialize * (IH (Pos.to_nat p - Pos.to_nat m') _ _ (coPset_sub1_helper C INF m)). *)
+  (*   { subst d. enough (Pos.to_nat m < Pos.to_nat m'); [lia| ]. *)
+  (*     apply Pos2Nat.inj_lt.  *)
+  (*     subst m m'. apply (coPset_nth_lt C INF 0 1). lia. } *)
+  (*   { apply elem_of_difference. split; auto.  *)
+  (*     apply not_elem_of_singleton. intros ->. lia. } *)
+  (*   { eauto. } *)
+  (*   { lia. } *)
+  (*   destruct IH as [n' EQ']. exists (S n'). simpl. set_solver. *)
+  (* Qed.        *)
+  Admitted. 
+
+End CoPsetOrdering.
