fairness/lawyer/action_model.v
@@ -1,0 +1,529 @@
+From trillium.fairness Require Import fairness.
+From trillium.fairness Require Import utils.
+From stdpp Require Import namespaces coPset. 
+From iris.proofmode Require Import proofmode.
+
+
+Import derived_laws_later.bi.
+
+Section Actions.
+  Definition Action := positive.
+
+  Definition pick_act `{Countable T} (pref: namespace) (t: T) :=
+    coPpick $ ↑ (pref .@ encode t).
+  Definition acts_at (pref: namespace): coPset := ↑ pref. 
+
+  Lemma pick_act_dom `{Countable T} ns (t: T):
+    pick_act ns t ∈ (↑ns: coPset). 
+  Proof.
+    rewrite /pick_act.
+    eapply elem_of_weaken; [apply coPpick_elem_of| ].
+    { apply nclose_infinite. }
+    apply nclose_subseteq.
+  Qed.
+    
+  Lemma pick_act_inj `{CNT: Countable T} pref: Inj eq eq (@pick_act _ _ CNT pref).
+  Proof.
+    red. rewrite /pick_act. intros ?? EQ.
+    destruct (decide (x = y)) as [| NEQ]; auto.
+    assert ((↑pref.@encode x: coPset) ## (↑pref.@encode y)) as D.
+    { assert (encode x ≠ encode y); [| solve_ndisj].
+      intros ?. destruct NEQ. eapply encode_inj; eauto. }
+  (*   opose proof * (coPpick_elem_of (↑pref.@encode x)) as IN1. *)
+  (*   { eapply nclose_infinite. } *)
+  (*   opose proof * (coPpick_elem_of (↑pref.@encode y)) as IN2. *)
+  (*   { eapply nclose_infinite. } *)
+  (*   rewrite EQ in IN1. set_solver. *)
+  (* Qed. *)
+  Admitted. 
+    
+  Lemma pick_act_disj_neq `{Countable T1} `{Countable T2}
+    ns1 ns2 (DISJ: ns1 ## ns2):
+    forall (a: T1) (b: T2), 
+      pick_act ns1 a ≠ pick_act ns2 b.
+  Proof.
+    intros.
+    pose proof (pick_act_dom ns1 a). pose proof (pick_act_dom ns2 b) as DOM2.
+    intros EQ. rewrite -EQ in DOM2.
+    edestruct DISJ; eauto. 
+  Qed. 
+
+  Lemma pick_act_notin_disj_ns `{Countable T}
+      ns ns' (DISJ: ns ## ns'):
+    forall (t: T), pick_act ns t ∉ (↑ ns': coPset).
+  Proof.
+    intros. apply disjoint_singleton_l.
+    symmetry. eapply disjoint_subseteq.
+    - apply _.
+    - reflexivity.
+    - apply elem_of_subseteq_singleton, pick_act_dom.
+    - done. 
+  Qed.
+
+  Lemma pick_act_ns_nth_disj_neq `{Countable T}
+    ns C INF (DISJ: ↑ ns ## C):
+    forall (a: T) n, pick_act ns a ≠ coPset_nth C INF n.
+  Proof.
+    intros.
+    pose proof (pick_act_dom ns a). pose proof (coPset_nth_in C INF n) as DOM2.
+    intros EQ. rewrite -EQ in DOM2.
+    edestruct DISJ; eauto. 
+  Qed.  
+
+End Actions.
+
+Section ActionModel.
+
+  Record ActionModel := {
+      amSt: Type;
+      amRole: Type;
+      amTrans: amSt -> Action * option amRole -> amSt -> Prop;
+
+      am_role_eqdec :> EqDecision amRole;
+      am_role_cnt :> Countable amRole;
+      am_st_eqdec :> EqDecision amSt;
+      am_st_inh :> Inhabited amSt;
+      am_role_inh :> Inhabited amRole;
+  }.
+
+  Arguments amTrans {_}.
+  Global Existing Instance am_role_eqdec. 
+  Global Existing Instance am_role_cnt. 
+  Global Existing Instance am_st_eqdec.
+  Global Existing Instance am_st_inh.
+  Global Existing Instance am_role_inh.
+ 
+
+  (* Defining the properites below as typeclasses to allow automatic inference *)
+  
+  (* similar to "live roles" of FairModel, but the roles are optional, 
+     and the list cannot contain anything non-stepping. *)
+  Class AM_strong_lr (AM: ActionModel) := {
+      ams_lr: amSt AM -> gset (option (amRole AM));
+      ams_lr_spec: forall st oρ, oρ ∈ ams_lr st <-> exists a st', amTrans st (a, oρ) st'
+  }.
+
+  Class AM_fin_branch (AM: ActionModel) := {
+      amfb_ns: amSt AM -> list (amSt AM * Action * option (amRole AM));
+      amfb_ns_spec: forall s1 s2 a oρ, amTrans s1 (a, oρ) s2 <-> (s2, a, oρ) ∈ amfb_ns s1
+  }. 
+
+  (* a weaker version of AM_fin_branch that is easier to show *)
+  Class AM_fin_branch' (AM: ActionModel) := {
+    amfb'_ns: amSt AM -> list (amSt AM * Action * option (amRole AM));
+    amfb'_ns_spec: forall s1 s2 a oρ, amTrans s1 (a, oρ) s2 -> (s2, a, oρ) ∈ amfb'_ns s1
+  }.
+
+  Class AM_step_dec (AM: ActionModel) :=
+    amsd: forall s1 a oρ s2, Decision (@amTrans AM s1 (a, oρ) s2). 
+
+  (* derive the strong finite branching from weaker one
+     by filtering possible transitions *)
+  Global Instance AM_fin_branch_dec (AM: ActionModel)
+    (FIN: AM_fin_branch' AM) (DEC: AM_step_dec AM):
+    AM_fin_branch AM.
+  Proof. 
+    destruct FIN as [ns' FIN]. 
+    exists (fun s => filter (fun '(s2, a, oρ) => @bool_decide _ (DEC s a oρ s2)) (ns' s)).
+    intros. rewrite elem_of_list_filter. rewrite bool_decide_spec.
+    symmetry. apply iff_and_impl_helper. intuition.
+  Qed.
+
+  (* TODO: move *)
+  Lemma ex_prod {A B: Type} (P: A * B -> Prop):
+    (exists ab, P ab) <-> (exists a b, P (a, b)).
+  Proof.
+    split.
+    - intros [[??] ?]. eauto.
+    - intros (?&?&?). eauto.
+  Qed. 
+
+  (* (optional) live roles can be obtained by checking all possible transitions,
+     given that there is a finite number of them *)
+  Global Instance fin_branch_strong (AM: ActionModel)
+    (FIN: AM_fin_branch AM):
+    AM_strong_lr AM.
+  Proof.
+    destruct FIN as [ns FIN]. 
+    exists (fun s => list_to_set ((fun '(_, _, oρ) => oρ) <$> ns s)). 
+    intros. rewrite elem_of_list_to_set. rewrite elem_of_list_fmap.
+    do 2 rewrite ex_prod.
+    setoid_rewrite ex_det_iff with (a := oρ); [| by intuition].
+    rewrite ex2_comm. do 2 (apply exist_proper; intros).
+    rewrite FIN. tauto.
+  Qed. 
+
+  (* useful for defining the set of _non-optional_ live_roles of AM *)
+  Definition extract_Somes {A: Type} (l: list (option A)): list A :=
+    flat_map (from_option (fun a => [a]) []) l.
+
+  Lemma extract_Somes_spec {A: Type} (l: list (option A)):
+    forall a, In (Some a) l <-> In a (extract_Somes l).
+  Proof. 
+    intros. rewrite /extract_Somes.
+    rewrite in_flat_map_Exists.
+    rewrite List.Exists_exists. simpl.
+    erewrite ex_det_iff with (a := Some a). 
+    2: { intros ? [? ?]. destruct a'; try done.
+         simpl in H0. set_solver. }
+    simpl. set_solver.
+  Qed.
+
+  Definition extract_Somes_gset `{Countable A} (s: gset (option A)): gset A :=
+    list_to_set ∘ extract_Somes ∘ elements $ s. 
+  
+  Lemma extract_Somes_gset_spec `{Countable A} (s: gset (option A)):
+    forall a, Some a ∈ s <-> a ∈ (extract_Somes_gset s).
+  Proof. 
+    intros. rewrite /extract_Somes_gset.
+    rewrite elem_of_list_to_set. 
+    rewrite elem_of_list_In. rewrite -extract_Somes_spec.
+    rewrite -elem_of_list_In. rewrite elem_of_elements.
+    done. 
+  Qed.
+
+  Lemma extract_Somes_gset_inv `{Countable A} (s: gset (option A)):
+    set_map Some (extract_Somes_gset s) = s ∖ {[ None ]}.
+  Proof. 
+    apply set_eq. intros ?. rewrite elem_of_map.
+    setoid_rewrite <- extract_Somes_gset_spec.
+    rewrite elem_of_difference not_elem_of_singleton.
+    split; [intros (?&->&?) | intros [??]]. 
+    - set_solver.
+    - destruct x; eauto. done.
+  Qed. 
+
+  (* the counterpart of FairModel's "live_roles" *)
+  Definition AM_live_roles `{AM_strong_lr AM}:
+    amSt AM -> gset (amRole AM) :=
+    extract_Somes_gset ∘ ams_lr. 
+
+  Lemma AM_live_roles_spec `{AM_strong_lr AM}:
+    forall st ρ,
+    (exists a st', amTrans st (a, Some ρ) st') <-> ρ ∈ AM_live_roles st.
+  Proof. 
+    intros. rewrite /AM_live_roles /compose.
+    rewrite -extract_Somes_gset_spec.
+    by rewrite ams_lr_spec. 
+  Qed.
+
+  Section ActionsOf.
+    Context (AM: ActionModel). 
+
+    Definition is_action_of (a: Action) := 
+      exists st oρ st', @amTrans AM st (a, oρ) st'.
+
+    Lemma action_of_step st a oρ st'
+      (STEP: @amTrans AM st (a, oρ) st'):
+      is_action_of a.
+    Proof. red. eauto. Qed.  
+
+  End ActionsOf.
+
+  Section AMProduct.
+    Context (AM1 AM2: ActionModel).
+    
+    Let PS: Type := @amSt AM1 * @amSt AM2.
+    Let PR: Type := @amRole AM1 + @amRole AM2.
+
+    Context
+      {is_act1_dec: forall a, Decision (is_action_of AM1 a)}
+      {is_act2_dec: forall a, Decision (is_action_of AM2 a)}.
+
+    Inductive ProdTrans: PS -> Action * option PR -> PS -> Prop :=
+    | pt_inner1 s1 s1' s2 a r1 
+        (NO2: ¬ is_action_of AM2 a)
+        (STEP1: amTrans s1 (a, Some r1) s1'):
+      ProdTrans (s1, s2) (a, Some (inl r1)) (s1', s2)
+    | pt_inner2 s2 s2' s1 a r2
+        (NO1: ¬ is_action_of AM1 a)
+        (STEP2: amTrans s2 (a, Some r2) s2'):
+      ProdTrans (s1, s2) (a, Some (inr r2)) (s1, s2')
+    | pt_sync1 s1 s1' s2 s2' a r1
+        (STEP1: amTrans s1 (a, Some r1) s1')
+        (STEP2: amTrans s2 (a, None) s2'):
+      ProdTrans (s1, s2) (a, Some (inl r1)) (s1', s2')
+    | pt_sync2 s1 s1' s2 s2' a r2
+        (STEP1: amTrans s1 (a, None) s1')
+        (STEP2: amTrans s2 (a, Some r2) s2'):
+      ProdTrans (s1, s2) (a, Some (inr r2)) (s1', s2')
+    | pt_sync_ext s1 s1' s2 s2' a
+        (STEP1: amTrans s1 (a, None) s1')
+        (STEP2: amTrans s2 (a, None) s2'):
+      ProdTrans (s1, s2) (a, None) (s1', s2')
+    .
+    
+    Definition ProdAM: ActionModel := {| amTrans := ProdTrans; |}.    
+
+    Global Instance prod_AM_step_dec {EQ1: EqDecision (amSt AM1)} {EQ2: EqDecision (amSt AM2)}
+      (D1: AM_step_dec AM1) (D2: AM_step_dec AM2)
+      :
+      AM_step_dec ProdAM.
+    Proof.
+      red. intros [s1 s2] a oρ [s1' s2'].
+      Ltac inv_step := right; intros S; inversion S; subst; congruence.
+      destruct oρ as [ρ| ].
+      2: { destruct (D1 s1 a None s1'), (D2 s2 a None s2').
+           all: try inv_step.
+           left. econstructor; eauto. }
+      destruct ρ as [ρ1 | ρ2]. 
+      - destruct (D1 s1 a (Some ρ1) s1'), (D2 s2 a None s2').
+        all: try inv_step.
+        + left. econstructor; eauto.
+        + destruct (is_act2_dec a), (decide (s2' = s2)) as [-> | ?].
+          all: try inv_step.
+          repeat econstructor; eauto.
+      - destruct (D1 s1 a None s1'), (D2 s2 a (Some ρ2) s2').
+        all: try inv_step.
+        + left. econstructor; eauto.
+        + destruct (is_act1_dec a), (decide (s1' = s1)) as [-> | ?].
+          all: try inv_step.
+          repeat econstructor; eauto.
+    Qed.
+
+    Global Instance prod_AM_fin_branch' (FIN1: AM_fin_branch' AM1) (FIN2: AM_fin_branch' AM2)
+      :
+      AM_fin_branch' ProdAM.
+    Proof. 
+      destruct FIN1 as [ns1 FIN1], FIN2 as [ns2 FIN2].
+      set (dummy := xH). 
+      exists (fun '(s1, s2) =>
+           '(s1', a1, oρ1) ← (s1, dummy, None) :: ns1 s1;
+           '(s2', a2, oρ2) ← (s2, dummy, None) :: ns2 s2;
+           a ← [a1; a2];
+           ρ' ← [from_option (Some ∘ inl) None oρ1; from_option (Some ∘ inr) None oρ2];
+           mret ((s1', s2'), a, ρ')). 
+           
+      intros [s1 s2] [s1' s2'] a oρ STEP.
+      rewrite elem_of_list_bind.
+      rewrite !ex_prod.
+
+      (* TODO: shorten the following proof, rewrite under binders? *)
+      (* setoid_rewrite elem_of_list_bind.       *)
+
+      (* do 3 (eapply exist_proper; intros). *)
+      (* { pattern x1. match goal with |- ((fun y => ?F y <-> _) x1) => idtac "foo" end.  *)      
+
+      inversion STEP; subst.
+      { exists s1', a, (Some r1).
+        split; [| set_solver]. 
+        rewrite elem_of_list_bind.
+        exists (s2', dummy, None). set_solver. }
+      { exists s1', dummy, None. 
+        split; [| set_solver]. 
+        rewrite elem_of_list_bind.
+        exists (s2', a, Some r2). set_solver. }
+      { exists s1', a, (Some r1).
+        split; [| set_solver]. 
+        rewrite elem_of_list_bind.
+        exists (s2', a, None). 
+        rewrite elem_of_list_bind. set_solver. }
+      { exists s1', a, None.
+        split; [| set_solver]. 
+        rewrite elem_of_list_bind.
+        exists (s2', a, Some r2). set_solver. }
+      { exists s1', a, None.
+        split; [| set_solver].
+        rewrite elem_of_list_bind.
+        exists (s2', a, None). set_solver. }
+    Qed.
+
+    Section Independent.
+
+      Class models_independent :=
+        mi_indep: forall a, is_action_of AM1 a -> is_action_of AM2 a -> False.
+
+      Context (INDEP: models_independent).
+
+      Lemma prod_indep_live_roles
+        (* `{AM_fin_branch' AM1} `{AM_step_dec AM1} `{EqDecision (amSt AM1)} *)
+        (* `{AM_fin_branch' AM2} `{AM_step_dec AM2} `{EqDecision (amSt AM2)} *)
+        `{AM_strong_lr AM1} `{AM_strong_lr AM2} `{AM_strong_lr ProdAM}
+        (st1: amSt AM1) (st2: amSt AM2):
+        AM_live_roles ((st1, st2): amSt ProdAM) = 
+        set_map inl (AM_live_roles st1) ∪ 
+        set_map inr (AM_live_roles st2).
+      Proof using INDEP.
+        simpl. rewrite set_eq. intros ?.
+        rewrite elem_of_union !elem_of_map.
+        rewrite -(@AM_live_roles_spec ProdAM).
+        repeat setoid_rewrite <- AM_live_roles_spec.
+        split.
+        { intros (a & st' & STEP). inversion STEP; subst.
+          all: set_solver. }
+        intros [(?&->&?&?&STEP)|(?&->&?&?&STEP)].
+        - do 2 eexists. apply pt_inner1; eauto.
+          intros ?. eapply INDEP; eauto.
+          eapply action_of_step; eauto. 
+        - do 2 eexists. apply pt_inner2; eauto.
+          intros ?. eapply INDEP; eauto.
+          eapply action_of_step; eauto.
+      Qed.
+        
+    End Independent.
+
+  End AMProduct.
+
+  Section AM2FM.
+    Context (AM: ActionModel).
+
+    (* this requirement is not necessary, but allows to reuse the AM_strong_lr machinery *)
+    Context (AM_S: AM_strong_lr AM). 
+
+    Inductive am_fmtrans: amSt AM → option (amRole AM) → amSt AM → Prop :=
+    | amfm_role_step s1 s2 a r (STEP: amTrans s1 (a, Some r) s2):
+      am_fmtrans s1 (Some r) s2
+    | amfm_env_step s1 s2 a (STEP: amTrans s1 (a, None) s2):
+      am_fmtrans s1 None s2
+    .
+
+    Lemma am_fmtrans_action s1 oρ s2:
+      am_fmtrans s1 oρ s2 <-> exists a, amTrans s1 (a, oρ) s2.
+    Proof.
+      split.
+      - intros STEP. inversion STEP; eauto.
+      - intros [a STEP]. destruct oρ; econstructor; eauto.
+    Qed. 
+
+    Definition AM2FM : FairModel.
+      refine {| fmtrans := am_fmtrans; live_roles := AM_live_roles |}.
+    Proof. 
+      intros. apply AM_live_roles_spec.
+      inversion H; eauto.
+    Defined. 
+
+  End AM2FM.
+
+End ActionModel.
+
+Section MatchedBy.
+
+  Definition synced_by {M__s M__m} 
+    (R: amSt M__s -> amSt M__m -> Prop)
+    := 
+    forall st__s st__s' a ρ st__m,
+      R st__s st__m -> is_action_of M__m a ->
+      amTrans _ st__s (a, Some ρ) st__s' -> 
+    exists st__m', amTrans _ st__m (a, None) st__m' /\ R st__s' st__m'.
+
+  Definition matched_by {M__s M__m} 
+    (R: amSt M__s -> amSt M__m -> Prop)
+    (L: amRole M__s -> amRole M__m)
+    := 
+    forall st__s st__s' a ρ st__m,
+      R st__s st__m -> 
+      amTrans _ st__s (a, Some ρ) st__s' -> 
+    exists st__m', amTrans _ st__m (a, Some $ L ρ) st__m' /\ R st__s' st__m'.
+
+  Lemma matched_by_prod_l {M__s M__m} R
+    {is_act_m_dec: forall a, Decision (is_action_of M__m a)}
+    (SYNC: synced_by R)
+    (PRIV_S_R: forall st__s st__s' a ρ st__m,
+        R st__s st__m -> amTrans _ st__s (a, Some ρ) st__s' -> ¬ (is_action_of M__m a) ->
+        R st__s' st__m)
+    :
+    @matched_by M__s (ProdAM M__s M__m)
+      (fun st__s '(st__s', st__m) => st__s' = st__s /\ R st__s st__m)
+      inl
+  .
+  Proof using.
+    red. intros st__s st__s' a ρ [? st__m]. intros [-> R1] STEP. 
+    destruct (decide (is_action_of M__m a)).
+    - unshelve epose proof (SYNC st__s) as (st__m' & STEP__m & R2);  eauto. 
+      (* opose proof * SYNC as (st__m' & STEP__m & R2); eauto. *)
+      eexists (_, _). split; eauto. econstructor; eauto.
+    - eexists (_, _). split; [| split]; [| reflexivity| eapply PRIV_S_R]; eauto.  
+      econstructor; eauto.
+  Qed. 
+
+  Lemma matched_by_prod_r {M__s M__m} R
+    {is_act_m_dec: forall a, Decision (is_action_of M__m a)}
+    (SYNC: synced_by R)
+    (PRIV_S_R: forall st__s st__s' a ρ st__m,
+        R st__s st__m -> amTrans _ st__s (a, Some ρ) st__s' -> ¬ (is_action_of M__m a) ->
+        R st__s' st__m):
+    @matched_by M__s (ProdAM M__m M__s)
+      (fun st__s '(st__m, st__s') => st__s' = st__s /\ R st__s st__m)
+      inr
+  . 
+  Proof using.
+    red. intros st__s st__s' a ρ [? st__m]. intros [-> R1] STEP. 
+    destruct (decide (is_action_of M__m a)).
+    -
+      epose proof (SYNC st__s) as (st__m' & STEP__m & R2); eauto.
+      eexists (_, _). split; eauto. econstructor; eauto.
+    - eexists (_, _). split; [| split]; [| reflexivity| eapply PRIV_S_R]; eauto.  
+      econstructor; eauto.
+  Qed.
+
+End MatchedBy.
+
+
+Section MatchedByFacts.
+  Context `(MATCH: @matched_by M__s M__m R L).
+
+  Lemma live_lift `{AM_strong_lr M__s} `{AM_strong_lr M__m}
+    ρ st__s st__m
+    (REL: R st__s st__m)
+    (LIVE: ρ ∈ AM_live_roles st__s)
+    :
+    L ρ ∈ AM_live_roles st__m. 
+  Proof using MATCH.
+    setoid_rewrite <- AM_live_roles_spec.
+    apply AM_live_roles_spec in LIVE. destruct LIVE as (?&?&STEP).
+    (* intros (ρ__e & -> & (a__e & st__e' & STEP__e)). *)
+    eapply MATCH in STEP; eauto. destruct STEP as (?&?&?). eauto. 
+  Qed.
+ 
+  Lemma matched_AM_live_roles `{AM_strong_lr M__s} `{AM_strong_lr M__m}
+    st__e st__o (R1: R st__e st__o):
+    set_map L (AM_live_roles st__e) ⊆ AM_live_roles st__o.
+  Proof using MATCH.
+    apply elem_of_subseteq. intros ρ (?&->&?)%elem_of_map.
+    eapply live_lift; eauto.
+  Qed.
+ 
+End MatchedByFacts.
+
+(* TODO: move all of this *)
+Definition UnitAM: ActionModel :=
+  {| amSt := unit; amRole := unit; amTrans := fun _ _ _ => False |}.
+
+Lemma matched_by_unit AM R:
+  @synced_by AM UnitAM R. 
+Proof. 
+  red. intros ?????? ACT.
+  red in ACT. set_solver.
+Qed. 
+
+Lemma unit_indep_r AM:
+  models_independent AM UnitAM.
+Proof. 
+  red. intros ?? ACT. red in ACT. set_solver.
+Qed.
+
+Lemma unit_indep_l AM:
+  models_independent UnitAM AM.
+Proof. 
+  red. intros ? ACT. red in ACT. set_solver.
+Qed.
+
+Global Instance UnitAM_step_dec: AM_step_dec UnitAM. 
+Proof. right. tauto. Qed.
+
+Global Instance UnitAM_fin_branch': AM_fin_branch' UnitAM.
+Proof. exists (fun _ => []). done. Qed. 
+
+Lemma unit_lr (st: amSt UnitAM):
+  AM_live_roles st = ∅.
+Proof. 
+  apply set_eq. intros. rewrite -AM_live_roles_spec. set_solver. 
+Qed. 
+
+Lemma UnitAM_actions a: is_action_of UnitAM a <-> False.
+Proof. split; [| done]. by intros (?&?&?&?). Qed. 
+
+
+(* Section AM2M. *)
+
+(* End  *)
