fairness/lawyer/sub_action_em.v
@@ -1,0 +1,114 @@
+From stdpp Require Import fin_maps.
+From iris.proofmode Require Import tactics.
+From trillium Require Import language.
+From trillium.program_logic Require Import traces weakestpre.
+From trillium.fairness Require Import locales_helpers execution_model.
+From trillium.fairness.lawyer Require Import action_model.
+
+
+Class ActionSubEM (Λ: language) (AM: ActionModel) := {
+
+    (* TODO: how to express that these two are typeclasses themselves? *)
+    asem_preGS: gFunctors -> Set;
+    asem_GS: gFunctors -> Set;
+    asem_Σ: gFunctors;
+    asem_Σ_subG: forall Σ, subG asem_Σ Σ -> asem_preGS Σ;
+
+    asem_valid_evolution_step:
+      cfg Λ -> olocale Λ → cfg Λ → 
+      amSt AM → Action * option (amRole AM) → amSt AM → Prop;
+
+    asem_msi {Σ} `{asem_GS Σ}: cfg Λ -> amSt AM -> iProp Σ;
+    
+    asem_init_param: Type; 
+    asem_init_resource {Σ: gFunctors} `{asem_GS Σ}: 
+      amSt AM → asem_init_param -> iProp Σ;
+    asem_is_init_st: cfg Λ -> amSt AM -> Prop;
+    
+    asem_initialization Σ `{ePreGS: asem_preGS Σ}: 
+    forall (s1: amSt AM) (σ: cfg Λ) (p: asem_init_param)
+      (INIT_ST: asem_is_init_st σ s1),
+      ⊢ (|==> ∃ eGS: asem_GS Σ, @asem_init_resource _ eGS s1 p ∗ @asem_msi _ eGS σ s1)
+}.
+
+(* TODO: move *)
+Definition AM2M (AM: ActionModel): Model := {| mtrans := amTrans AM |}.
+
+
+Definition TopAM_EM {Λ AM} (ASEM: ActionSubEM Λ AM)
+  (thread_post: forall Σ, asem_GS Σ -> locale Λ → iProp Σ):
+  ExecutionModel Λ (AM2M AM).
+  esplit. 
+  - apply asem_Σ_subG.
+  - apply asem_valid_evolution_step.
+  - exact thread_post. 
+  - by apply asem_initialization.
+Defined. 
+  
+Section AM_UPD.
+
+  Context `{ASEM: ActionSubEM Λ AM}. 
+  Context `{aeGS: asem_GS Σ}.
+  Context `{Countable (locale Λ)}.
+  
+  Definition AM_st_interp_interim (c c': cfg Λ)
+    (δ: amSt AM) (τ: locale Λ) oτ': iProp Σ :=
+    asem_msi c δ (asem_GS0 := aeGS) ∗ 
+    ⌜ locale_step c (Some τ) c' ⌝ ∗
+    ⌜ step_fork c c' = oτ' ⌝
+  .
+
+  Section AMU.
+    Context {iGS: invGS_gen HasNoLc Σ}. 
+
+    Definition AMU_impl
+      (f: option (locale Λ)) E ζ (a: Action) (P : iProp Σ): iProp Σ :=
+      ∀ c c' δ, 
+        AM_st_interp_interim c c' δ ζ f ={E}=∗
+        ∃ δ' oρ, asem_msi c' δ' (asem_GS0 := aeGS) ∗
+                 (* ⌜ amTrans _ δ (a, oρ) δ' ⌝ ∗ P *)
+                 ⌜ asem_valid_evolution_step c (Some ζ) c' δ (a, oρ) δ' ⌝ ∗
+                 P
+    .
+
+    Definition AMU := AMU_impl None.
+    Definition AMU__f E ζ ζ' P := AMU_impl (Some ζ') E ζ P. 
+
+  End AMU.
+
+End AM_UPD.
+
+
+Section AMU_HL.
+  From trillium.fairness.lawyer Require Import program_logic. 
+    
+  Context `{ASEM: ActionSubEM heap_lang AM}. 
+  Context {Σ: gFunctors}. 
+
+  Definition AMU_lift_MU
+    `{aeGS: asem_GS Σ}
+    `{EM: ExecutionModel heap_lang M} `{hGS: @heapGS Σ _ EM}
+    (A: coPset) := 
+    ⊢ ∀ E ζ P (a: Action) (Aa: a ∈ A), AMU E ζ a P (aeGS := aeGS) -∗ MU E ζ P.
+  
+  Lemma AMU_lift_top thread_post
+    (EM := TopAM_EM ASEM thread_post)
+    `{hGS: @heapGS Σ _ EM}
+    (aeGS := heap_fairnessGS (heapGS := hGS))
+    :
+    @AMU_lift_MU aeGS _ EM _ (↑ nroot).
+  Proof using.
+    red. iIntros (E ζ P ??). rewrite /AMU /AMU_impl /MU /MU_impl.
+    simpl. 
+    iIntros "AMU" (extr mtr) "TI'".
+    simpl. destruct extr as [| extr c']; [done| ]. simpl.
+    iDestruct "TI'" as "(?&MSI&->&%&%)".
+    iMod ("AMU" with "[MSI]") as "AMU".
+    { iFrame. iPureIntro. eauto. }
+    iModIntro. iDestruct "AMU" as (??) "(?&%&?)".
+    do 2 iExists _. iFrame. eauto.
+  Qed. 
+
+End AMU_HL.
+
+
